model/aws-sdk/kms/README.md
@@ -3,3 +3,4 @@ This is the KMS smithy model, but with a couple adjustments:
 - `com.amazonaws.kms#TrentService` is renamed to `com.amazonaws.kms#KeyManagementService`.
 - The `ListKeysResponse` structure is removed from the model.
 - The `ListKeys` operation is removed from the model, and from `com.amazon.kms#KeyManagementService`.
+- The `EncryptionContextKey` and `EncryptionContextValue` have the `aws.polymorph#dafnyUtf8Bytes` trait added.
